veric/MemoryPushouts.v
@@ -137,6 +137,7 @@ Qed.
 Lemma mem_unchanged_on_refl: forall m f, mem_unchanged_on f m m.
 Proof. intros. split; intros; trivial. Qed.
 
+(*
 Module PUSHOUTS.
 (*
 Require Import veric.Address.
@@ -343,3 +344,399 @@ exists m2',  Mem.inject j' m1' m2' /\ mem_forward m2 m2' /\
 Admitted.
 End PO_IE.
 End PUSHOUTS.
+*)
+
+Lemma po_trans: forall a b c, Mem.perm_order'' a b ->  Mem.perm_order'' b c ->
+      Mem.perm_order'' a c.
+Proof. intros.
+   destruct a; destruct b; destruct c; simpl in *; try contradiction; try trivial.
+   eapply perm_order_trans; eassumption.
+Qed.
+
+Lemma extends_perm: forall m1 m2 (Ext: Mem.extends m1 m2) b ofs k p,
+   Mem.perm m1 b ofs k p -> Mem.perm m2 b ofs k p.  
+Proof. intros. destruct Ext. destruct mext_inj.
+  specialize (mi_perm b b 0 ofs k p (eq_refl _) H).
+  rewrite Zplus_0_r in mi_perm. assumption.
+Qed.
+
+Lemma extends_permorder: forall m1 m2 (Ext: Mem.extends m1 m2) b ofs k,
+  Mem.perm_order'' (ZMap.get b (Mem.mem_access m2) ofs k)
+                   (ZMap.get b (Mem.mem_access m1) ofs k).
+Proof.
+  intros. destruct Ext.  destruct mext_inj as [prm _ _].
+  specialize (prm b b 0 ofs k). unfold Mem.perm in prm. 
+  remember ((ZMap.get b (Mem.mem_access m2) ofs k)) as z.
+  destruct z; apply eq_sym in Heqz; simpl  in *. 
+    remember ((ZMap.get b (Mem.mem_access m1) ofs k)) as zz.
+    destruct zz; trivial; apply eq_sym in Heqzz; simpl  in *.
+       rewrite Zplus_0_r in prm. rewrite Heqz in prm. 
+       specialize (prm p0 (eq_refl _)). apply prm. apply perm_refl. 
+  remember ((ZMap.get b (Mem.mem_access m1) ofs k)) as zz.
+    destruct zz; trivial; apply eq_sym in Heqzz; simpl  in *.
+       rewrite Zplus_0_r in prm. rewrite Heqz in prm. 
+       specialize (prm p (eq_refl _)). exfalso. apply prm. apply perm_refl. 
+Qed.
+
+Lemma fwd_maxperm: forall m1 m2 (FWD: mem_forward m1 m2) b 
+  (V:Mem.valid_block m1 b) ofs p,
+  Mem.perm m2 b ofs Max p -> Mem.perm m1 b ofs Max p.
+Proof. intros. apply FWD; assumption. Qed. 
+
+Lemma fwd_maxpermorder: forall m1 m2 (FWD: mem_forward m1 m2) b 
+  (V:Mem.valid_block m1 b) ofs,
+  Mem.perm_order'' (ZMap.get b (Mem.mem_access m1) ofs Max)
+                   (ZMap.get b (Mem.mem_access m2) ofs Max).
+Proof.
+  intros. destruct (FWD b); try assumption. 
+  remember ((ZMap.get b (Mem.mem_access m2) ofs Max)) as z.
+  destruct z; apply eq_sym in Heqz; simpl  in *.
+  remember ((ZMap.get b (Mem.mem_access m1) ofs Max)) as zz.
+  destruct zz; apply eq_sym in Heqzz; simpl  in *.
+  specialize (H0 ofs p).  unfold Mem.perm in H0. unfold Mem.perm_order' in H0. 
+  rewrite Heqz in H0. rewrite Heqzz in H0. apply H0. apply perm_refl.
+  specialize (H0 ofs p).  unfold Mem.perm in H0. unfold Mem.perm_order' in H0. 
+  rewrite Heqz in H0. rewrite Heqzz in H0. apply H0. apply perm_refl.
+
+
+  remember ((ZMap.get b (Mem.mem_access m1) ofs Max)) as zz.
+  destruct zz; apply eq_sym in Heqzz; simpl in *; trivial.
+Qed.
+
+Lemma po_oo: forall p q, Mem.perm_order' p q = Mem.perm_order'' p (Some q).
+Proof. intros. destruct p; trivial. Qed. 
+
+Lemma load_E: forall (chunk: memory_chunk) (m: mem) (b: block) (ofs: Z),
+  Mem.load chunk m b ofs = 
+  if Mem.valid_access_dec m chunk b ofs Readable
+  then Some(decode_val chunk (Mem.getN (size_chunk_nat chunk) ofs ((ZMap.get b m.(Mem.mem_contents)))))
+  else None.
+Proof. intros. reflexivity. Qed.
+
+Definition AccessMap_EE_Property  (m1 m1' m2 m3':Mem.mem) 
+           (AM:ZMap.t (Z -> perm_kind -> option permission)):Prop :=
+  forall b, 
+    (Mem.valid_block m2 b -> forall k ofs,
+         (Mem.perm m1 b ofs Max Nonempty ->
+          ZMap.get b AM ofs k = ZMap.get b m1'.(Mem.mem_access) ofs k) /\ 
+         (~Mem.perm m1 b ofs Max Nonempty ->
+          ZMap.get b AM ofs k = ZMap.get b m2.(Mem.mem_access) ofs k))
+     /\ (~ Mem.valid_block m2 b -> forall k ofs,
+           ZMap.get b AM ofs k = ZMap.get b m3'.(Mem.mem_access) ofs k).
+
+Definition ContentMap_EE_Property (m1 m2 m3':Mem.mem) (CM:ZMap.t (ZMap.t memval)) :=
+  forall b,
+    (Mem.valid_block m2 b -> forall ofs,
+         (Mem.perm m1 b ofs Max Nonempty ->
+          ZMap.get ofs (ZMap.get b CM) = ZMap.get ofs (ZMap.get b m3'.(Mem.mem_contents))) /\ 
+         (~Mem.perm m1 b ofs Max Nonempty ->
+          ZMap.get ofs (ZMap.get b CM) = ZMap.get ofs (ZMap.get b m2.(Mem.mem_contents))))
+     /\ (~ Mem.valid_block m2 b -> forall ofs,
+           ZMap.get ofs (ZMap.get b CM) = ZMap.get ofs (ZMap.get b m3'.(Mem.mem_contents))).
+
+Lemma EE_ok: forall (m1 m1' m2 m3 m3':Mem.mem) (Ext12: Mem.extends m1 m2) (Fwd1: mem_forward m1 m1')
+             (Ext23: Mem.extends m2 m3) (Fwd3: mem_forward m3 m3') (Ext13' : Mem.extends m1' m3')
+             (UnchOn13 :  mem_unchanged_on (loc_out_of_bounds m1) m3 m3')
+(*also have this premise: (UnchOn23 :  mem_unchanged_on (loc_out_of_bounds m2) m3 m3')*)
+             m2'
+             (NB: m2'.(Mem.nextblock)=m3'.(Mem.nextblock))
+(*             (CONT:  ContentMap_EE_Property m1 m2 m3' (m2'.(Mem.mem_contents))) *)
+             (CONT: Mem.mem_contents m2' = Mem.mem_contents m3')
+             (MaxAccess: AccessMap_EE_Property  m1 m1' m2 m3' (m2'.(Mem.mem_access))),
+               mem_forward m2 m2' /\ Mem.extends m1' m2' /\ Mem.extends m2' m3' /\
+                          mem_unchanged_on (loc_out_of_bounds m1) m2 m2'.
+Proof. intros.
+assert (Fwd2: mem_forward m2 m2').
+    split; intros.
+     (*valid_block*) apply (Mem.valid_block_extends _ _ b Ext23) in H. 
+        apply Fwd3 in H. destruct H as[H _]. 
+        unfold Mem.valid_block. rewrite NB. apply H.
+      (*max*)
+        destruct (MaxAccess b) as [X _].
+        unfold Mem.perm in *. destruct (X H Max ofs). clear X MaxAccess.
+        remember (Mem.perm_order'_dec (ZMap.get b (Mem.mem_access m1) ofs Max) Nonempty) as d.
+        destruct d; clear Heqd.  
+           clear H2. rewrite (H1 p0) in H0. clear H1. 
+           rewrite po_oo in *.
+           assert (ZZ:= fwd_maxpermorder _ _ Fwd1).
+           apply (Mem.valid_block_extends _ _ b Ext12) in H. 
+           assert (XX:= extends_permorder _ _ Ext12 b ofs Max).
+           eapply po_trans. apply XX.
+           eapply po_trans. apply (ZZ _ H). apply H0.
+        clear H1. rewrite (H2 n) in H0. apply H0. 
+split; trivial.
+assert (Ext12':  Mem.extends m1' m2').  
+    split. 
+    (*nextblock*)
+        rewrite NB. apply Ext13'.
+    (*mem_inj*)
+       split; intros.
+         (*mi_perm*)
+            destruct k.
+            (*MAX*)
+              destruct (MaxAccess b1) as [Val Inval].
+              unfold Mem.perm. rewrite po_oo.
+              inv H. rewrite Zplus_0_r.
+              remember (zlt b2 (Mem.nextblock m2)) as z.
+              destruct z. clear Inval. destruct (Val z Max ofs); clear Val Heqz. 
+                remember (Mem.perm_dec m1 b2 ofs Max Nonempty) as d. 
+                destruct d; clear Heqd.  
+                   clear H1. rewrite (H p0). apply H0. 
+                clear H. rewrite (H1 n).
+                   assert (ZZ:= fwd_maxpermorder _ _ Fwd1).
+                   assert (XX:= extends_permorder _ _ Ext12 b2 ofs Max).
+                   apply (Mem.valid_block_extends _ _ b2 Ext12) in z. 
+                   eapply po_trans. apply XX.
+                   eapply po_trans. apply (ZZ _ z). apply H0.
+              clear Val. rewrite (Inval z).
+                 eapply po_trans. apply (extends_permorder _ _ Ext13').
+                                  apply H0.
+             (*CUR*)
+              destruct (MaxAccess b2) as [Val Inval].
+              inv H. rewrite Zplus_0_r.
+              remember (zlt b2 (Mem.nextblock m2)) as z.
+              destruct z. clear Inval. destruct (Val z Cur ofs); clear Val Heqz. 
+                remember (Mem.perm_dec m1 b2 ofs Max Nonempty) as d. 
+                destruct d; clear Heqd.  
+                   clear H1. unfold Mem.perm. rewrite (H p0). apply H0. 
+                clear H. unfold Mem.perm. rewrite (H1 n). clear H1.
+                   apply Mem.perm_max in H0.
+                   apply (Mem.valid_block_extends _ _ b2 Ext12) in z. 
+                   assert (ZZ:= fwd_maxperm _ _ Fwd1 _ z _ _ H0).
+                   exfalso. apply n. eapply Mem.perm_implies. apply ZZ. apply perm_any_N.
+              clear Val. unfold Mem.perm. rewrite po_oo in *. 
+                 rewrite (Inval z Cur). clear Inval.
+                 eapply po_trans. apply (extends_permorder _ _ Ext13').
+                                  apply H0.
+         (*mi_access*) unfold Mem.valid_access in *. destruct H0. inv H. rewrite Zplus_0_r.
+             split; trivial. 
+             intros off; intros. specialize (H0 _ H). 
+              destruct (MaxAccess b2) as [Val Inval].
+              remember (zlt b2 (Mem.nextblock m2)) as z.
+              destruct z. clear Inval. destruct (Val z Cur off); clear Val Heqz. 
+                remember (Mem.perm_dec m1 b2 off Max Nonempty) as d. 
+                destruct d; clear Heqd.  
+                   clear H1. unfold Mem.perm. rewrite (H2 p0). apply H0. 
+                clear H. unfold Mem.perm. rewrite (H3 n). clear H1.
+                   apply Mem.perm_max in H0.
+                   apply (Mem.valid_block_extends _ _ b2 Ext12) in z. 
+                   assert (ZZ:= fwd_maxperm _ _ Fwd1 _ z _ _ H0).
+                   exfalso. apply n. eapply Mem.perm_implies. apply ZZ. apply perm_any_N.
+              clear Val. unfold Mem.perm. rewrite po_oo in *. 
+                 rewrite (Inval z Cur). clear Inval.
+                 eapply po_trans. apply (extends_permorder _ _ Ext13').
+                                  apply H0.
+         (*mi_memval *) inv H. rewrite Zplus_0_r. rewrite CONT.
+            destruct Ext13'. destruct mext_inj as [_ _ X]. 
+            specialize (X b2 _ _ _ (refl_equal _) H0). rewrite Zplus_0_r in X. 
+            apply X. 
+split; trivial.
+assert (Ext23': Mem.extends m2' m3').
+    split. 
+    (*nextblock*)
+        apply NB. 
+    (*mem_inj*)
+       split; intros.
+         (*mi_perm*)
+            destruct k.
+            (*MAX*)
+              destruct (MaxAccess b1) as [Val Inval].
+              inv H. rewrite Zplus_0_r.
+              remember (zlt b2 (Mem.nextblock m2)) as z.
+              destruct z. clear Inval. destruct (Val z Max ofs);  clear Val.
+                remember (Mem.perm_dec m1 b2 ofs Max Nonempty) as d.
+                destruct d; clear Heqd.  
+                   clear H1. unfold Mem.perm in *. rewrite (H p0) in H0. clear H p0.
+                   destruct Ext13'. destruct mext_inj as [mperm _ _].
+                   unfold Mem.perm in mperm. 
+                   specialize (mperm b2 b2 0 ofs Max p (eq_refl _)).
+                   rewrite Zplus_0_r in mperm. 
+                   apply mperm. apply H0.
+                clear H. unfold Mem.perm in *. rewrite (H1 n) in H0. clear H1.
+                   eapply UnchOn13. apply n.
+                   destruct Ext23. destruct mext_inj as [mperm _ _].
+                   apply (mperm b2 b2 0) in H0. rewrite Zplus_0_r in H0. assumption.
+                        reflexivity.
+              clear Val. unfold Mem.perm in H0. rewrite (Inval z Max ofs) in H0. apply H0.
+             (*CUR*)
+              destruct (MaxAccess b2) as [Val Inval].
+              inv H. rewrite Zplus_0_r.
+              remember (zlt b2 (Mem.nextblock m2)) as z.
+              destruct z. clear Inval. destruct (Val z Cur ofs); clear Val Heqz. 
+                remember (Mem.perm_dec m1 b2 ofs Max Nonempty) as d. 
+                destruct d; clear Heqd.  
+                   clear H1. unfold Mem.perm in *. rewrite po_oo in *. 
+                   rewrite (H p0) in H0; clear H. 
+                   eapply po_trans. eapply (extends_permorder _ _ Ext13' b2 ofs Cur).
+                   apply H0. 
+                clear H. 
+                   eapply UnchOn13. apply n.
+                   unfold Mem.perm in *. rewrite po_oo in *. 
+                   rewrite (H1 n) in H0; clear H1. 
+                   apply (Mem.valid_block_extends _ _ b2 Ext23) in z. 
+                   eapply po_trans. apply (extends_permorder _ _ Ext23 b2 ofs Cur). 
+                       apply H0. 
+              clear Val. unfold Mem.perm in *. rewrite po_oo in *. 
+                 rewrite (Inval z Cur) in H0. clear Inval. apply H0.
+         (*mi_access*) unfold Mem.valid_access in *. destruct H0. inv H. rewrite Zplus_0_r.
+             split; trivial. 
+             intros off; intros. specialize (H0 _ H). clear H.
+              destruct (MaxAccess b2) as [Val Inval].
+              remember (zlt b2 (Mem.nextblock m2)) as z.
+              destruct z. clear Inval. destruct (Val z Cur off); clear Val Heqz. 
+                remember (Mem.perm_dec m1 b2 off Max Nonempty) as d. 
+                destruct d; clear Heqd.  
+                   clear H1. unfold Mem.perm in *. rewrite po_oo in *. 
+                   rewrite (H p0) in H0; clear H. 
+                   eapply po_trans. eapply (extends_permorder _ _ Ext13' b2 off Cur).
+                   apply H0. 
+                clear H. 
+                   eapply UnchOn13. apply n.
+                   unfold Mem.perm in *. rewrite po_oo in *. 
+                   rewrite (H2 n) in H0; clear H2. 
+                   apply (Mem.valid_block_extends _ _ b2 Ext23) in z. 
+                   eapply po_trans. apply (extends_permorder _ _ Ext23 b2 off Cur). 
+                       apply H0. 
+              clear Val. unfold Mem.perm in *. rewrite po_oo in *. 
+                 rewrite (Inval z Cur) in H0. clear Inval. apply H0.
+         (*mi_memval *) inv H. rewrite Zplus_0_r. rewrite CONT. 
+            assert (ZZ: Mem.perm m3' b2 ofs Cur Readable). 
+               destruct (MaxAccess b2) as [Val Inval].
+               remember (zlt b2 (Mem.nextblock m2)) as z.
+               destruct z. clear Inval. destruct (Val z Cur ofs); clear Val Heqz. 
+                 remember (Mem.perm_dec m1 b2 ofs Max Nonempty) as d. 
+                 destruct d; clear Heqd.  
+                    clear H1. unfold Mem.perm in *. rewrite po_oo in *. 
+                    rewrite (H p) in H0; clear H. 
+                    eapply po_trans. apply (extends_permorder _ _ Ext13'). apply H0. 
+                 clear H. unfold Mem.perm in *. rewrite (H1 n) in H0. clear H1.
+                   eapply UnchOn13. apply n.
+                   unfold Mem.perm. rewrite po_oo in *.  
+                   eapply po_trans. apply (extends_permorder _ _ Ext23). apply H0.
+               clear Val. unfold Mem.perm in *. rewrite po_oo in *. 
+                  rewrite (Inval z) in H0. apply H0.
+assert (WD: mem_wd m3'). admit.
+                  destruct WD as [_ _ X].
+                  assert (VAL:= Mem.perm_valid_block _ _ _  _ _ ZZ). 
+                  assert (VV: Mem.flat_inj (Mem.nextblock m3') b2 = Some (b2, 0)). 
+                    unfold Mem.flat_inj. unfold Mem.valid_block in VAL. 
+                    destruct (zlt b2  (Mem.nextblock m3')). trivial.
+                     clear - z VAL. exfalso. omega. 
+                  specialize (X b2 ofs b2 0 VV ZZ). rewrite Zplus_0_r in *.
+                  destruct X. constructor.
+                    apply flatinj_E in H. destruct H as [? [? ?]]; subst.
+                    econstructor. reflexivity. repeat rewrite Int.add_zero. trivial. 
+                    destruct mv; try econstructor.
+                       reflexivity. repeat rewrite Int.add_zero. trivial. 
+split; trivial.
+(*mem_unchanged_on (loc_out_of_bounds m1) m2 m2'*)
+     destruct UnchOn13 as [Unch1 Unch2].
+     split; intros. clear Unch2.
+        unfold loc_out_of_bounds in *.
+        assert (XX:= extends_perm _ _ Ext23 _ _ _ _ H0).
+        specialize (Unch1 _ _ k p H XX). 
+          destruct (MaxAccess b) as [Val _].
+          unfold Mem.perm.
+          destruct (Val (Mem.perm_valid_block _ _ _ _ _ H0) k ofs) as [_ X]; clear Val.  
+          rewrite (X H); clear X. apply H0. 
+   admit. (*ToDo: explore whether ContentMap_EE_Property works
+      rewrite load_E.
+      destruct (MaxAccess b) as [Val Inval]. rewrite load_E in *. clear Unch1 Unch2.
+        unfold loc_out_of_bounds in *.
+        remember (Mem.valid_access_dec m2 chunk b ofs Readable) as z.
+        destruct z. inv H0. destruct v0. unfold Mem.range_perm in *.
+          assert (BValid2: Mem.valid_block m2 b).
+            eapply Mem.perm_valid_block. apply (r ofs). 
+               split. omega. destruct chunk; simpl; omega. 
+          clear Inval; specialize (Val BValid2). 
+          remember (Mem.valid_access_dec m2' chunk b ofs Readable) as zz. 
+          destruct zz. xx Print size_chunk.     specialize (Val _ 
+      assert (X: Mem.load chunk m3' b ofs = Some v). 
+        apply (Unch2 _ _ _ v H). clear Unch2 MaxAccess H. 
+        assert (XX:= Mem.load_extends _ _ _ _ _ _ Ext23 H0).
+        rewrite load_E in *. 
+        remember (Mem.valid_access_dec m2 chunk b ofs Readable) as z.
+        destruct z; inv H0. 
+        destruct Ext23. destruct mext_inj.
+           clear Heqz. apply (mi_access b b 0) in v0; try reflexivity.
+           rewrite Zplus_0_r in *. 
+           remember (Mem.valid_access_dec m3 chunk b ofs Readable) as zz.
+             destruct zz. Focus 2. exfalso. apply (n v0). SearchAbout Mem.load. 
+             unfold Mem.getN. inv H0. 
+      assert (X: Mem.load chunk m3' b ofs = Some v). 
+      rewrite load_E in *. 
+        remember (Mem.valid_access_dec m2 chunk b ofs Readable) as z.
+        destruct z. unfold Mem.valid_access in v0. inv H0; clear Heqz. destruct v0. admit. *)
+Qed.
+ 
+Parameter mkAccessMap_EE_exists: 
+           forall (m1 m1' m2 m3':Mem.mem), ZMap.t (Z -> perm_kind -> option permission).
+Axiom mkAccessMap_EE_ok: forall m1 m1' m2 m3', 
+      AccessMap_EE_Property m1 m1' m2 m3' (mkAccessMap_EE_exists m1 m1' m2 m3').
+
+Definition mkEE (m1 m1' m2 m3 m3':Mem.mem) (Ext12: Mem.extends m1 m2) (Fwd1: mem_forward m1 m1')
+                (Ext23: Mem.extends m2 m3) (Fwd3: mem_forward m3 m3') (Ext13' : Mem.extends m1' m3')
+                (UnchOn3: mem_unchanged_on (loc_out_of_bounds m1) m3 m3') : Mem.mem'.
+eapply Mem.mkmem with (nextblock:=m3'.(Mem.nextblock))
+                      (mem_access:=mkAccessMap_EE_exists m1 m1' m2 m3').
+(* (NB: forall b, Mem.valid_block m2 b -> Mem.valid_block m3' b)*)
+  apply m3'.(Mem.mem_contents).
+  apply m3'.
+  (*access_max*)
+  intros. destruct (mkAccessMap_EE_ok m1 m1' m2 m3' b) as [Val Inval].
+    remember (zlt b m2.(Mem.nextblock)) as z. 
+    destruct z; clear Heqz.
+    (*Case valid*) clear Inval.
+        specialize (Val z). 
+        destruct (Val Max ofs) as [MaxA MaxB].
+        destruct (Val Cur ofs) as [CurA CurB]. clear Val. 
+        remember (Mem.perm_dec m1 b ofs Max Nonempty) as zz.
+        destruct zz; clear Heqzz.
+          rewrite (CurA p). rewrite (MaxA p). apply m1'.
+          rewrite (CurB n). rewrite (MaxB n). apply m2. (*apply m3'.*)
+    (*Case invalid*) clear Val.
+        specialize (Inval z). 
+        rewrite (Inval Max ofs).
+        rewrite (Inval Cur ofs). apply m3'. 
+  (*nextblock_noaccess*)
+    intros.  destruct (mkAccessMap_EE_ok m1 m1' m2 m3' b) as [_ Inval].
+    rewrite Inval. apply m3'. apply H. 
+    clear Inval Ext12 Fwd1 Ext13'. intros N. destruct Ext23. 
+      unfold mem_forward, Mem.valid_block in *. 
+      rewrite mext_next in N.
+      apply Fwd3 in N.  destruct N as [X _]. clear - H X. omega.
+Defined.
+
+Lemma interpolate_EE: forall m1 m2 (Ext12: Mem.extends m1 m2) m1' 
+            (Fwd1: mem_forward m1 m1') m3 (Ext23: Mem.extends m2 m3) m3' 
+            (Fwd3: mem_forward m3 m3') (Ext13' : Mem.extends m1' m3')
+            (UnchOn3: mem_unchanged_on (loc_out_of_bounds m1) m3 m3'),
+       exists m2', mem_forward m2 m2' /\ Mem.extends m1' m2' /\ Mem.extends m2' m3' /\
+                          mem_unchanged_on (loc_out_of_bounds m1) m2 m2'.
+Proof. intros.
+   assert (NB:forall b, Mem.valid_block m2 b -> Mem.valid_block m3' b).
+      intros. apply Fwd3. destruct Ext23. unfold Mem.valid_block. rewrite <- mext_next. apply H.
+   exists (mkEE m1 m1' m2 m3 m3' Ext12 Fwd1 Ext23 Fwd3 Ext13' UnchOn3).
+     eapply (EE_ok m1 m1' m2 m3 m3'); trivial.
+     apply mkAccessMap_EE_ok.  
+Qed. 
+
+Lemma interpolate_EI: forall (m1 m2 m1':mem) (Ext12: Mem.extends m1 m2) (Fwd1: mem_forward m1 m1')
+                              m3 j (Ext23: Mem.inject j m2 m3) m3' (Fwd3: mem_forward m3 m3') j'
+                             (Inj13': Mem.inject j' m1' m3')
+                             (UnchOn3: mem_unchanged_on (loc_out_of_reach j m1) m3 m3') 
+                             (InjInc: inject_incr j j') (injSep: inject_separated j j' m1 m3)
+                             (UnchOn1: mem_unchanged_on (loc_unmapped j) m1 m1'),
+       exists m2', mem_forward m2 m2' /\ Mem.extends m1' m2' /\ Mem.inject j' m2' m3' /\ 
+                   mem_unchanged_on (loc_out_of_bounds m1) m2 m2' /\
+                   mem_unchanged_on (loc_unmapped j) m2 m2'.
+Admitted. 
+
+Lemma interpolate_IE: forall m1 m1' m2 j (Minj12 : Mem.inject j m1 m2) (Fwd1: mem_forward m1 m1') 
+                             j' (InjInc: inject_incr j j')  (Sep12 : inject_separated j j' m1 m2) 
+                             (UnchLUj: mem_unchanged_on (loc_unmapped j) m1 m1')
+                             m3 m3' (Ext23 : Mem.extends m2 m3) (Fwd3: mem_forward m3 m3') 
+                             (UnchLOORj1_3: mem_unchanged_on (loc_out_of_reach j m1) m3 m3'),
+                 exists m2', Mem.inject j' m1' m2' /\ mem_forward m2 m2' /\ Mem.extends m2' m3' /\
+                             mem_unchanged_on (loc_out_of_reach j m1) m2 m2'.                                         
+Admitted.
